src/opt/Compatibility.v
@@ -4,7 +4,7 @@ Require Import List.
 
 Require Import sflib.
 Require Import paco.
-Require Import respectful5.
+Require Import respectful7.
 
 Require Import Axioms.
 Require Import Basic.
@@ -27,10 +27,9 @@ Definition SIM_REGS := forall (rs_src rs_tgt:RegFile.t), Prop.
 
 Inductive sim_terminal
           (sim_regs:SIM_REGS)
-          (th_src th_tgt:Thread.t lang): Prop :=
+          (st_src:lang.(Language.state)) (st_tgt:lang.(Language.state)): Prop :=
 | sim_terminal_intro
-    (REGS: sim_regs th_src.(Thread.state).(State.regs) th_tgt.(Thread.state).(State.regs))
-    (COMMIT: Commit.le th_src.(Thread.commit) th_tgt.(Thread.commit))
+    (REGS: sim_regs st_src.(State.regs) st_tgt.(State.regs))
 .
 
 Definition sim_expr
@@ -50,17 +49,17 @@ Definition _sim_stmts
     (PROMISE: MemInv.sem Memory.bot promise_src promise_tgt),
     sim_thread
       (sim_terminal sim_regs1)
-      (Thread.mk lang (State.mk rs_src stmts_src) commit_src promise_src) mem_k_src
-      (Thread.mk lang (State.mk rs_tgt stmts_tgt) commit_tgt promise_tgt) mem_k_tgt.
+      (State.mk rs_src stmts_src) (Thread.mk commit_src promise_src) mem_k_src
+      (State.mk rs_tgt stmts_tgt) (Thread.mk commit_tgt promise_tgt) mem_k_tgt.
 
 Lemma _sim_stmts_mon
-      s1 s2 (S: s1 <5= s2):
+      s1 s2 (S: s1 <7= s2):
   _sim_stmts s1 <4= _sim_stmts s2.
 Proof.
   ii. apply S. apply PR; auto.
 Qed.
 
-Lemma step_seq
+Lemma lang_step_seq
       stmts rs1 stmts1 rs2 stmts2 e
       (STEP: State.step (State.mk rs1 stmts1) e
                         (State.mk rs2 stmts2)):
@@ -73,7 +72,7 @@ Proof.
   - s. rewrite <- app_assoc. econs 3.
 Qed.
 
-Lemma step_deseq
+Lemma lang_step_deseq
       stmts rs1 stmt1 stmts1 rs2 stmts2 e
       (STEP: State.step (State.mk rs1 (stmt1 :: stmts1 ++ stmts)) e
                         (State.mk rs2 stmts2)):
@@ -92,89 +91,63 @@ Lemma internal_step_seq
       stmts
       rs1 stmts1 commit1 promise1 mem1
       rs2 stmts2 commit2 promise2 mem2
-      (STEP: Thread.internal_step
-               (Thread.mk lang (State.mk rs1 stmts1) commit1 promise1) mem1
-               (Thread.mk lang (State.mk rs2 stmts2) commit2 promise2) mem2):
-  Thread.internal_step
-    (Thread.mk lang (State.mk rs1 (stmts1 ++ stmts)) commit1 promise1) mem1
-    (Thread.mk lang (State.mk rs2 (stmts2 ++ stmts)) commit2 promise2) mem2.
+      (STEP: Executor.internal_step
+               (Executor.mk lang (State.mk rs1 stmts1) (Thread.mk commit1 promise1) mem1)
+               (Executor.mk lang (State.mk rs2 stmts2) (Thread.mk commit2 promise2) mem2)):
+  Executor.internal_step
+    (Executor.mk lang (State.mk rs1 (stmts1 ++ stmts)) (Thread.mk commit1 promise1) mem1)
+    (Executor.mk lang (State.mk rs2 (stmts2 ++ stmts)) (Thread.mk commit2 promise2) mem2).
 Proof.
-  inv STEP.
+  inv STEP; ss.
   - econs 1; s; eauto.
-  - econs 2; s; eauto. apply step_seq. auto.
-  - econs 3; s; eauto. apply step_seq. auto.
-  - econs 4; s; eauto. apply step_seq. auto.
-  - econs 5; s; eauto. apply step_seq. auto.
-  - econs 6; s; eauto. apply step_seq. auto.
+  - econs 2; s; eauto. apply lang_step_seq. auto.
+  - econs 3; s; eauto. apply lang_step_seq. auto.
 Qed.
 
-Lemma thread_step_seq
+Lemma step_seq
       stmts e
       rs1 stmts1 commit1 promise1 mem1
       rs2 stmts2 commit2 promise2 mem2
-      (STEP: Thread.step e
-               (Thread.mk lang (State.mk rs1 stmts1) commit1 promise1) mem1
-               (Thread.mk lang (State.mk rs2 stmts2) commit2 promise2) mem2):
-  Thread.step e
-    (Thread.mk lang (State.mk rs1 (stmts1 ++ stmts)) commit1 promise1) mem1
-    (Thread.mk lang (State.mk rs2 (stmts2 ++ stmts)) commit2 promise2) mem2.
+      (STEP: Executor.step
+               (Executor.mk lang (State.mk rs1 stmts1) (Thread.mk commit1 promise1) mem1) e
+               (Executor.mk lang (State.mk rs2 stmts2) (Thread.mk commit2 promise2) mem2)):
+  Executor.step
+    (Executor.mk lang (State.mk rs1 (stmts1 ++ stmts)) (Thread.mk commit1 promise1) mem1) e
+    (Executor.mk lang (State.mk rs2 (stmts2 ++ stmts)) (Thread.mk commit2 promise2) mem2).
 Proof.
-  inv STEP.
-  - econs 1. eapply internal_step_seq. auto.
-  - econs 2; eauto. inv STATE. econs; eauto.
-Qed.
-
-Lemma _internal_step_seq
-      stmts
-      rs1 stmts1 commit1 promise1 mem1
-      rs2 stmts2 commit2 promise2 mem2
-      (STEP: Thread._internal_step
-               (Thread.mk lang (State.mk rs1 stmts1) commit1 promise1, mem1)
-               (Thread.mk lang (State.mk rs2 stmts2) commit2 promise2, mem2)):
-  Thread._internal_step
-    (Thread.mk lang (State.mk rs1 (stmts1 ++ stmts)) commit1 promise1, mem1)
-    (Thread.mk lang (State.mk rs2 (stmts2 ++ stmts)) commit2 promise2, mem2).
-Proof.
-  inv STEP. econs. ss.
-  apply internal_step_seq. auto.
+  inv STEP; ss.
+  - econs 1. apply internal_step_seq. auto.
+  - econs 2. inv STEP0. econs; ss. apply lang_step_seq. auto.
 Qed.
 
 Lemma thread_step_deseq
       stmts e
       rs1 stmt1 stmts1 commit1 promise1 mem1
       rs2 stmts2 commit2 promise2 mem2
-      (STEP: Thread.step e
-                         (Thread.mk lang (State.mk rs1 (stmt1 :: stmts1 ++ stmts)) commit1 promise1) mem1
-                         (Thread.mk lang (State.mk rs2 stmts2) commit2 promise2) mem2):
+      (STEP: Executor.step
+               (Executor.mk lang (State.mk rs1 (stmt1 :: stmts1 ++ stmts)) (Thread.mk commit1 promise1) mem1) e
+               (Executor.mk lang (State.mk rs2 stmts2) (Thread.mk commit2 promise2) mem2)):
   exists stmts2',
     stmts2 = stmts2' ++ stmts /\
-  Thread.step e
-              (Thread.mk lang (State.mk rs1 (stmt1 :: stmts1)) commit1 promise1) mem1
-              (Thread.mk lang (State.mk rs2 stmts2') commit2 promise2) mem2.
+  Executor.step
+    (Executor.mk lang (State.mk rs1 (stmt1 :: stmts1)) (Thread.mk commit1 promise1) mem1) e
+    (Executor.mk lang (State.mk rs2 stmts2') (Thread.mk commit2 promise2) mem2).
 Proof.
   inv STEP.
   - inv STEP0; ss.
     + rewrite app_comm_cons.
       eexists. splits; eauto.
       econs 1. econs 1; s; eauto.
-    + apply step_deseq in STATE. des. subst.
+    + apply lang_step_deseq in STATE. des. subst.
       eexists. splits; eauto.
       econs 1. econs 2; s; eauto.
-    + apply step_deseq in STATE. des. subst.
+    + apply lang_step_deseq in STATE. des. subst.
       eexists. splits; eauto.
       econs 1. econs 3; s; eauto.
-    + apply step_deseq in STATE. des. subst.
-      eexists. splits; eauto.
-      econs 1. econs 4; s; eauto.
-    + apply step_deseq in STATE. des. subst.
-      eexists. splits; eauto.
-      econs 1. econs 5; s; eauto.
-    + apply step_deseq in STATE. des. subst.
-      eexists. splits; eauto.
-      econs 1. econs 6; s; eauto.
-  - inv STATE.
+  - inv STEP0. ss.
+    apply lang_step_deseq in STATE. des. subst.
     eexists. splits; eauto.
-    econs 2; eauto. econs; eauto.
+    econs 2. econs; s; eauto.
 Qed.
 
 Lemma sim_rtc
@@ -197,42 +170,39 @@ Proof.
     econs; eauto.
 Qed.
 
-Inductive sim_seq (s:list Stmt.t): forall (lhs rhs:Thread.t lang * Memory.t), Prop :=
+Inductive sim_seq (s:list Stmt.t): forall (lhs rhs:Executor.t lang), Prop :=
 | sim_seq_intro
     rs stmts commit promise mem:
     sim_seq s
-            (Thread.mk lang (State.mk rs stmts) commit promise, mem)
-            (Thread.mk lang (State.mk rs (stmts ++ s)) commit promise, mem)
+            (Executor.mk lang (State.mk rs stmts) (Thread.mk commit promise) mem)
+            (Executor.mk lang (State.mk rs (stmts ++ s)) (Thread.mk commit promise) mem)
 .
 
 Lemma rtc_internal_step_seq
       stmts
       rs1 stmts1 commit1 promise1 mem1
       rs2 stmts2 commit2 promise2 mem2
-      (STEP: rtc (@Thread._internal_step lang)
-               (Thread.mk lang (State.mk rs1 stmts1) commit1 promise1, mem1)
-               (Thread.mk lang (State.mk rs2 stmts2) commit2 promise2, mem2)):
-  rtc (@Thread._internal_step lang)
-    (Thread.mk lang (State.mk rs1 (stmts1 ++ stmts)) commit1 promise1, mem1)
-    (Thread.mk lang (State.mk rs2 (stmts2 ++ stmts)) commit2 promise2, mem2).
+      (STEP: rtc (@Executor.internal_step lang)
+                 (Executor.mk lang (State.mk rs1 stmts1) (Thread.mk commit1 promise1) mem1)
+                 (Executor.mk lang (State.mk rs2 stmts2) (Thread.mk commit2 promise2) mem2)):
+  rtc (@Executor.internal_step lang)
+      (Executor.mk lang (State.mk rs1 (stmts1 ++ stmts)) (Thread.mk commit1 promise1) mem1)
+      (Executor.mk lang (State.mk rs2 (stmts2 ++ stmts)) (Thread.mk commit2 promise2) mem2).
 Proof.
   exploit (sim_rtc (sim_seq stmts)); eauto.
-  - i. inv SIM1. inv RA. ss.
-    destruct a2. destruct t. destruct state. ss.
-    exploit _internal_step_seq; eauto. i.
+  - i. inv SIM1. destruct a2. destruct state. destruct thread.
+    generalize (internal_step_seq stmts RA). i.
     eexists. splits; eauto. econs; eauto.
   - econs; eauto.
   - i. des. inv x1. auto.
-Unshelve.
-  { econs; auto. }
 Qed.
 
 Inductive ctx (sim_thread:SIM_THREAD lang lang): SIM_THREAD lang lang :=
 | ctx_incl
     sim_terminal
-    th1 mem_k_src th2 mem_k_tgt
-    (SIM: sim_thread sim_terminal th1 mem_k_src th2 mem_k_tgt):
-    ctx sim_thread sim_terminal th1 mem_k_src th2 mem_k_tgt
+    st1 th1 mem_k_src st2 th2 mem_k_tgt
+    (SIM: sim_thread sim_terminal st1 th1 mem_k_src st2 th2 mem_k_tgt):
+    ctx sim_thread sim_terminal st1 th1 mem_k_src st2 th2 mem_k_tgt
 | ctx_nil
     (sim_regs:SIM_REGS)
     rs_src mem_k_src
@@ -244,8 +214,8 @@ Inductive ctx (sim_thread:SIM_THREAD lang lang): SIM_THREAD lang lang :=
     (PROMISE: MemInv.sem Memory.bot promise_src promise_tgt):
     ctx sim_thread
         (sim_terminal sim_regs)
-        (Thread.mk lang (State.mk rs_src []) commit_src promise_src) mem_k_src
-        (Thread.mk lang (State.mk rs_tgt []) commit_tgt promise_tgt) mem_k_tgt
+        (State.mk rs_src []) (Thread.mk commit_src promise_src) mem_k_src
+        (State.mk rs_tgt []) (Thread.mk commit_tgt promise_tgt) mem_k_tgt
 | ctx_instr
     instr regs
     rs_src mem_k_src
@@ -258,20 +228,20 @@ Inductive ctx (sim_thread:SIM_THREAD lang lang): SIM_THREAD lang lang :=
     (PROMISE: MemInv.sem Memory.bot promise_src promise_tgt):
     ctx sim_thread
         (sim_terminal (RegFile.eq_except regs))
-        (Thread.mk lang (State.mk rs_src [Stmt.instr instr]) commit_src promise_src) mem_k_src
-        (Thread.mk lang (State.mk rs_tgt [Stmt.instr instr]) commit_tgt promise_tgt) mem_k_tgt
+        (State.mk rs_src [Stmt.instr instr]) (Thread.mk commit_src promise_src) mem_k_src
+        (State.mk rs_tgt [Stmt.instr instr]) (Thread.mk commit_tgt promise_tgt) mem_k_tgt
 | ctx_seq
     sim_regs1 sim_regs2
     stmts1_src stmts2_src rs_src commit_src promise_src mem_k_src
     stmts1_tgt stmts2_tgt rs_tgt commit_tgt promise_tgt mem_k_tgt
     (SIM1: sim_thread (sim_terminal sim_regs1)
-                      (Thread.mk lang (State.mk rs_src stmts1_src) commit_src promise_src) mem_k_src
-                      (Thread.mk lang (State.mk rs_tgt stmts1_tgt) commit_tgt promise_tgt) mem_k_tgt)
+                      (State.mk rs_src stmts1_src) (Thread.mk commit_src promise_src) mem_k_src
+                      (State.mk rs_tgt stmts1_tgt) (Thread.mk commit_tgt promise_tgt) mem_k_tgt)
     (SIM2: _sim_stmts sim_thread sim_regs1 stmts2_src stmts2_tgt sim_regs2):
     ctx sim_thread
         (sim_terminal sim_regs2)
-        (Thread.mk lang (State.mk rs_src (stmts1_src ++ stmts2_src)) commit_src promise_src) mem_k_src
-        (Thread.mk lang (State.mk rs_tgt (stmts1_tgt ++ stmts2_tgt)) commit_tgt promise_tgt) mem_k_tgt
+        (State.mk rs_src (stmts1_src ++ stmts2_src)) (Thread.mk commit_src promise_src) mem_k_src
+        (State.mk rs_tgt (stmts1_tgt ++ stmts2_tgt)) (Thread.mk commit_tgt promise_tgt) mem_k_tgt
 | ctx_ite
     sim_regs0 sim_regs1
     cond_src stmts1_src stmts2_src rs_src mem_k_src
@@ -286,8 +256,8 @@ Inductive ctx (sim_thread:SIM_THREAD lang lang): SIM_THREAD lang lang :=
     (SIM2: _sim_stmts sim_thread sim_regs0 stmts2_src stmts2_tgt sim_regs1):
     ctx sim_thread
         (sim_terminal sim_regs1)
-        (Thread.mk lang (State.mk rs_src [Stmt.ite cond_src stmts1_src stmts2_src]) commit_src promise_src) mem_k_src
-        (Thread.mk lang (State.mk rs_tgt [Stmt.ite cond_tgt stmts1_tgt stmts2_tgt]) commit_tgt promise_tgt) mem_k_tgt
+        (State.mk rs_src [Stmt.ite cond_src stmts1_src stmts2_src]) (Thread.mk commit_src promise_src) mem_k_src
+        (State.mk rs_tgt [Stmt.ite cond_tgt stmts1_tgt stmts2_tgt]) (Thread.mk commit_tgt promise_tgt) mem_k_tgt
 | ctx_dowhile
     sim_regs
     cond_src stmts_src rs_src mem_k_src
@@ -301,12 +271,12 @@ Inductive ctx (sim_thread:SIM_THREAD lang lang): SIM_THREAD lang lang :=
     (SIM: _sim_stmts sim_thread sim_regs stmts_src stmts_tgt sim_regs):
     ctx sim_thread
         (sim_terminal sim_regs)
-        (Thread.mk lang (State.mk rs_src [Stmt.dowhile stmts_src cond_src]) commit_src promise_src) mem_k_src
-        (Thread.mk lang (State.mk rs_tgt [Stmt.dowhile stmts_tgt cond_tgt]) commit_tgt promise_tgt) mem_k_tgt
+        (State.mk rs_src [Stmt.dowhile stmts_src cond_src]) (Thread.mk commit_src promise_src) mem_k_src
+        (State.mk rs_tgt [Stmt.dowhile stmts_tgt cond_tgt]) (Thread.mk commit_tgt promise_tgt) mem_k_tgt
 .
 Hint Constructors ctx.
 
-Lemma ctx_mon: monotone5 ctx.
+Lemma ctx_mon: monotone7 ctx.
 Proof.
   ii. inv IN.
   - econs 1. auto.
@@ -318,17 +288,17 @@ Proof.
 Qed.
 Hint Resolve ctx_mon.
 
-Lemma ctx_weak_respectful: weak_respectful5 (@_sim_thread lang lang) ctx.
+Lemma ctx_weak_respectful: weak_respectful7 (@_sim_thread lang lang) ctx.
 Proof.
   econs; auto. i. destruct PR.
   - (* incl *)
     eapply _sim_thread_mon; eauto.
-    apply rclo5_incl.
+    apply rclo7_incl.
   - (* nil *)
     ii.
     exploit MemInv.sem_bot_inv; eauto. i. subst.
     splits; s; i.
-    { inv TERMINAL_TGT. ss. eexists _, _. splits; eauto; ss. }
+    { inv TERMINAL_TGT. ss. eexists _, _, _. splits; eauto; ss. }
     { eexists. splits; try reflexivity; eauto.
       - etransitivity; eauto. apply Memory.splits_future. inv MEMORY. auto.
       - inv WF_SRC0. inv WF_TGT. ss. econs; ss.
@@ -337,24 +307,24 @@ Proof.
         apply Memory.splits_future. inv MEMORY. auto.
     }
     { ss. subst. eexists _, _. splits; eauto. }
-    inv STEP_TGT; ss.
-    + inv STEP; try inv STATE. ss.
-      exploit MemInv.promise; try apply MEMORY0; eauto.
-      { apply WF_SRC. }
-      { apply WF_TGT. }
-      s. i. des. apply MemInv.sem_bot_inv in INV2. subst.
-      exploit Memory.promise_future; try apply PROMISE_SRC; eauto.
-      { inv WF_SRC. auto. }
-      i. des.
-      eexists _, _, _, _. splits; eauto.
-      * instantiate (1 := Thread.mk _ _ _ _).
-        econs 1. econs 1; s; eauto.
-        inv WF_TGT. eapply Commit.future_wf; eauto.
-        etransitivity; eauto.
-        apply Memory.splits_future. inv MEMORY. auto.
-      * apply rclo5_step. apply ctx_nil; auto.
-        apply MemInv.sem_bot.
-    + inv STATE.
+    inv STEP_TGT; [|by inv STEP; inv STATE].
+    inv STEP; ss; try by inv STATE.
+    inv STEP0. ss.
+    exploit MemInv.promise; try apply MEMORY; eauto.
+    { apply WF_SRC. }
+    { apply WF_TGT. }
+    i. des. apply MemInv.sem_bot_inv in INV2. subst.
+    exploit Memory.promise_future; try apply PROMISE_SRC; eauto.
+    { inv WF_SRC. auto. }
+    { inv WF_SRC. auto. }
+    i. des.
+    eexists _, _, _, _, _, _. splits; eauto.
+    + econs 1. econs 1. s. econs; s; eauto.
+      inv WF_TGT. eapply Commit.future_wf; eauto.
+      etransitivity; eauto.
+      apply Memory.splits_future. inv MEMORY. auto.
+    + apply rclo7_step. apply ctx_nil; auto.
+      apply MemInv.sem_bot.
   - (* instr *)
     ii.
     exploit MemInv.sem_bot_inv; eauto. i. subst.
@@ -369,148 +339,154 @@ Proof.
     }
     { ss. subst. eexists _, _. splits; eauto. }
     inv STEP_TGT; ss.
-    + inv STEP; ss; try inv STATE.
-      * exploit MemInv.promise; try apply MEMORY0; eauto.
+    + inv STEP; inv STEP0; try inv STATE; ss.
+      * (* promise *)
+        exploit MemInv.promise; try apply MEMORY; eauto.
         { apply WF_SRC. }
         { apply WF_TGT. }
         s. i. des. apply MemInv.sem_bot_inv in INV2. subst.
         exploit Memory.promise_future; try apply PROMISE_SRC; eauto.
         { apply WF_SRC. }
+        { apply WF_SRC. }
         i. des.
-        eexists _, _, _, _. splits; eauto.
-        { instantiate (1 := Thread.mk _ _ _ _).
-          econs 1. econs 1; s; eauto.
+        eexists _, _, _, _, _, _. splits; eauto.
+        { econs 1. econs 1. econs; s; eauto.
           eapply Commit.future_wf; try apply WF_TGT; eauto.
           etransitivity; eauto. apply Memory.splits_future. inv MEMORY. eauto.
         }
-        { apply rclo5_step. apply ctx_instr; auto.
+        { apply rclo7_step. apply ctx_instr; auto.
           apply MemInv.sem_bot.
         }
-      * exploit RegFile.eq_except_instr; eauto. i. des.
-        generalize GET. intro X. apply MEMORY in X.
-        eexists _, _, _, _. splits; eauto.
-        { econs 1. econs 2; eauto. econs; eauto.
-          - s. eapply CommitFacts.read_mon; eauto.
-          - eapply Commit.future_wf; eauto.
-            apply Memory.splits_future. inv MEMORY. auto.
+      * (* silent *)
+        exploit RegFile.eq_except_instr; eauto. i. des.
+        eexists _, _, _, _, _, _. splits; eauto.
+        { econs 1. econs 2; ss.
+          - econs; eauto.
+          - econs; eauto.
+            eapply Commit.future_wf; try apply WF_TGT; eauto.
+            apply Memory.splits_future. inv MEMORY. eauto.
         }
-        { apply rclo5_step. apply ctx_nil; auto. reflexivity. }
-      * exploit RegFile.eq_except_instr; eauto. i. des.
+        { apply rclo7_step. apply ctx_nil; auto. }
+      * (* read *)
+        exploit RegFile.eq_except_instr; eauto. i. des.
+        generalize GET. intro X. apply MEMORY in X.
+        eexists _, _, _, _, _, _. splits; eauto.
+        { econs 1. econs 3; ss.
+          - econs. eauto.
+          - econs 1; eauto.
+            + s. eapply CommitFacts.read_mon; eauto.
+            + eapply Commit.future_wf; eauto.
+              apply Memory.splits_future. inv MEMORY. auto.
+        }
+        { apply rclo7_step. apply ctx_nil; auto. reflexivity. }
+      * (* write *)
+        exploit RegFile.eq_except_instr; eauto. i. des.
         exploit MemInv.write; try apply MEMORY0; eauto.
         { apply WF_SRC. }
         { apply WF_TGT. }
         i. des. apply MemInv.sem_bot_inv in INV2. subst.
-        eexists _, _, _, _. splits; eauto.
-        { econs 1. econs 3; ss; eauto. econs; eauto.
-          - s. eapply CommitFacts.write_mon; eauto.
-          - eapply Commit.future_wf; eauto.
-            apply Memory.splits_future. inv SIM2. auto.
+        eexists _, _, _, _, _, _. splits; eauto.
+        { econs 1. econs 3; ss.
+          - econs. eauto.
+          - econs 2; eauto.
+            + s. eapply CommitFacts.write_mon; eauto.
+            + eapply Commit.future_wf; eauto.
+              apply Memory.splits_future. inv SIM2. auto.
         }
-        { apply rclo5_step. apply ctx_nil; auto. reflexivity.
+        { apply rclo7_step. apply ctx_nil; auto. reflexivity.
           apply MemInv.sem_bot.
         }
-      * exploit RegFile.eq_except_instr; eauto. i. des.
+      * (* update *)
+        exploit RegFile.eq_except_instr; eauto. i. des.
         generalize GET. intro X. apply MEMORY in X.
         exploit MemInv.write; try apply MEMORY0; eauto.
         { apply WF_SRC. }
         { apply WF_TGT. }
         i. des. apply MemInv.sem_bot_inv in INV2. subst.
-        eexists _, _, _, _. splits; eauto.
-        { econs 1. econs 4; eauto. econs; eauto.
-          - s. eapply CommitFacts.read_mon; eauto.
-          - eapply Commit.future_wf; eauto.
-            apply Memory.splits_future. inv SIM2. auto.
+        eexists _, _, _, _, _, _. splits; eauto.
+        { econs 1. econs 3; ss.
+          - econs. eauto.
+          - econs 3; eauto.
+            + s. eapply CommitFacts.read_mon; eauto.
+            + eapply Commit.future_wf; eauto.
+              apply Memory.splits_future. inv SIM2. auto.
         }
-        { apply rclo5_step. apply ctx_nil; auto. reflexivity.
+        { apply rclo7_step. apply ctx_nil; auto. reflexivity.
           apply MemInv.sem_bot.
         }
-      * exploit RegFile.eq_except_instr; eauto. i. des.
-        eexists _, _, _, _. splits; eauto.
-        { econs 1. econs 5; eauto. econs; eauto.
-          - s. eapply CommitFacts.fence_mon; eauto.
-          - eapply Commit.future_wf; eauto.
-            apply Memory.splits_future. inv MEMORY. auto.
+      * (* fence *)
+        exploit RegFile.eq_except_instr; eauto. i. des.
+        eexists _, _, _, _, _, _. splits; eauto.
+        { econs 1. econs 3; ss.
+          - econs. eauto.
+          - econs 4; eauto.
+            + s. eapply CommitFacts.fence_mon; eauto.
+            + eapply Commit.future_wf; eauto.
+              apply Memory.splits_future. inv MEMORY. auto.
         }
-        { apply rclo5_step. apply ctx_nil; auto. reflexivity. }
-      * exploit RegFile.eq_except_instr; eauto. i. des.
-        eexists _, _, _, _. splits; eauto.
-        { econs 1. econs 6; eauto. econs; eauto.
+        { apply rclo7_step. apply ctx_nil; auto. reflexivity. }
+    + (* external *)
+      inv STEP. inv STEP0. inv STATE. ss.
+      exploit RegFile.eq_except_instr; eauto. i. des.
+      eexists _, _, _, _, _, _. splits; eauto.
+      * econs 2. econs; ss.
+        { econs. eauto. }
+        { econs; eauto.
           eapply Commit.future_wf; try apply WF_TGT; eauto.
           apply Memory.splits_future. inv MEMORY. eauto.
         }
-        { apply rclo5_step. apply ctx_nil; auto. }
-    + inv STATE.
-      exploit RegFile.eq_except_instr; eauto. i. des.
-      eexists _, _, _, _. splits; eauto.
-      * econs 2; eauto. econs; eauto.
-        eapply Commit.future_wf; try apply WF_TGT; eauto.
-        apply Memory.splits_future. inv MEMORY. eauto.
-      * apply rclo5_step. apply ctx_nil; auto.
+      * apply rclo7_step. apply ctx_nil; auto.
   - (* seq *)
     ii. ss.
-    exploit GF; eauto.
-    { econs; apply WF_SRC. }
-    { econs; apply WF_TGT. }
-    s. i. des.
+    exploit GF; eauto. s. i. des.
     splits; s; i.
     { inv TERMINAL_TGT. destruct stmts1_tgt, stmts2_tgt; inv H0.
       exploit TERMINAL; try by econs. i. des.
       exploit MemInv.sem_bot_inv; eauto. i. subst.
-      destruct th2_src, state. inv TERMINAL_SRC. ss. subst.
-      exploit Thread.rtc_internal_step_future; eauto; s.
-      { econs; apply WF_SRC. }
-      s. i. des.
+      destruct st2_src. inv TERMINAL_SRC. ss. subst.
+      exploit Executor.rtc_internal_step_future; eauto. s. i. des.
       inv SIM. ss. subst.
       exploit SIM2; eauto. intro TH2.
       exploit GF; eauto.
       { econs; apply WF2. }
       s. i. des.
       exploit TERMINAL0; try by econs. i. des.
-      destruct th2_src, state. inv TERMINAL_SRC. ss. subst.
-      eexists _, _. splits; [|eauto| | |eauto].
+      destruct st2_src, th2_src. inv TERMINAL_SRC. ss. subst.
+      eexists _, _, _. splits; [|eauto| |eauto|eauto|eauto].
       + etransitivity; [|eauto].
-        eapply rtc_internal_step_seq in STEPS. apply STEPS.
+        eapply rtc_internal_step_seq in STEPS. eauto.
       + econs.
-      + ss.
     }
-    { exploit FUTURE; eauto.
-      { econs; apply WF_SRC0. }
-      i. des. eexists. splits; eauto.
-      econs; apply WF_TGT0.
-    }
+    { eapply FUTURE; eauto. }
     { subst. exploit PROMISE; eauto. i. des.
-      destruct th2_src, state. ss. subst.
-      eexists _, _. splits; [|eauto|eauto].
-      + eapply rtc_internal_step_seq. apply STEPS.
-      + eauto.
+      destruct st2_src, th2_src. ss. subst.
+      eexists _, _, _. splits; [|eauto|eauto].
+      - eapply rtc_internal_step_seq. apply STEPS.
+      - ss.
     }
     destruct stmts1_tgt.
     + exploit TERMINAL; try by econs. i. des.
       exploit MemInv.sem_bot_inv; eauto. i. subst.
-      destruct th2_src, state. inv TERMINAL_SRC. ss. subst.
-      exploit Thread.rtc_internal_step_future; eauto; s.
-      { econs; apply WF_SRC. }
-      s. i. des.
+      destruct st2_src, th2_src. inv TERMINAL_SRC. ss. subst.
+      exploit Executor.rtc_internal_step_future; eauto. s. i. des.
       inv SIM. ss. subst.
       exploit SIM2; eauto. intro TH2.
-      exploit GF; eauto.
-      { econs; apply WF2. }
-      s. i. des.
+      exploit GF; eauto. s. i. des.
       exploit STEP0; eauto. i. des.
-      eexists _, _, _, _. splits; [|eauto|eauto|].
+      eexists _, _, _, _, _, _. splits; [|eauto|eauto|].
       * eapply rtc_internal_step_seq in STEPS.
         etransitivity; [apply STEPS|eauto].
-      * apply rclo5_incl. auto.
-    + destruct th3_tgt, state.
+      * apply rclo7_incl. auto.
+    + destruct st3_tgt, th3_tgt.
       exploit thread_step_deseq; eauto. i. des. ss. subst.
       exploit STEP; eauto. i. des.
-      destruct th2_src, state. destruct th3_src, state.
-      eexists _, _, _, _. splits; [| |eauto|].
+      destruct st2_src, th2_src. destruct st3_src, th3_src.
+      eexists _, _, _, _, _, _. splits; [| |eauto|].
       * eapply rtc_internal_step_seq. eauto.
-      * eapply thread_step_seq. eauto.
-      * apply rclo5_step. eapply ctx_seq; eauto.
-        { apply rclo5_incl. eauto. }
-        { eapply _sim_stmts_mon; try apply rclo5_incl; eauto.
+      * eapply step_seq. eauto.
+      * apply rclo7_step. eapply ctx_seq; eauto.
+        { apply rclo7_incl. eauto. }
+        { eapply _sim_stmts_mon; try apply rclo7_incl; eauto.
           eapply _sim_stmts_mon; try apply LE; eauto.
         }
   - (* ite *)
@@ -527,39 +503,41 @@ Proof.
     }
     { ss. subst. eexists _, _. splits; eauto. }
     inv STEP_TGT; ss.
-    + inv STEP; ss; try inv STATE.
-      * exploit MemInv.promise; try apply MEMORY0; eauto.
+    + inv STEP; inv STEP0; try inv STATE; ss.
+      * (* promise *)
+        exploit MemInv.promise; try apply MEMORY; eauto.
         { apply WF_SRC. }
         { apply WF_TGT. }
         s. i. des. apply MemInv.sem_bot_inv in INV2. subst.
         exploit Memory.promise_future; try apply PROMISE_SRC; eauto.
-        { inv WF_SRC. auto. }
+        { apply WF_SRC. }
+        { apply WF_SRC. }
         i. des.
-        eexists _, _, _, _. splits; eauto.
-        { instantiate (1 := Thread.mk _ _ _ _).
-          econs 1. econs 1; s; eauto.
+        eexists _, _, _, _, _, _. splits; eauto.
+        { econs 1. econs 1. econs; s; eauto.
           eapply Commit.future_wf; try apply WF_TGT; eauto.
           etransitivity; eauto. apply Memory.splits_future. inv MEMORY. eauto.
         }
-        { apply rclo5_step. eapply ctx_ite; eauto.
+        { apply rclo7_step. eapply ctx_ite; eauto.
           - apply MemInv.sem_bot.
-          - eapply _sim_stmts_mon; try apply rclo5_incl; eauto.
+          - eapply _sim_stmts_mon; try apply rclo7_incl; eauto.
             eapply _sim_stmts_mon; try apply LE; eauto.
-          - eapply _sim_stmts_mon; try apply rclo5_incl; eauto.
+          - eapply _sim_stmts_mon; try apply rclo7_incl; eauto.
             eapply _sim_stmts_mon; try apply LE; eauto.
         }
-      * eexists _, _, _, _. splits; try apply MEMORY; eauto.
-        { econs 1. econs 6; eauto. econs.
+      * (* ite *)
+        eexists _, _, _, _, _, _. splits; try apply MEMORY; eauto.
+        { econs 1. econs 2. econs; eauto. s. econs; eauto.
           eapply Commit.future_wf; try apply WF_TGT; eauto.
           apply Memory.splits_future. inv MEMORY. eauto.
         }
         { s. rewrite ? app_nil_r.
           exploit COND; eauto. intro C. rewrite C.
           destruct (RegFile.eval_expr rs_tgt cond_tgt).
-          - apply rclo5_incl. eauto.
-          - apply rclo5_incl. eauto.
+          - apply rclo7_incl. eauto.
+          - apply rclo7_incl. eauto.
         }
-    + inv STATE.
+    + inv STEP. inv STATE.
   - (* dowhile *)
     ii.
     exploit MemInv.sem_bot_inv; eauto. i. subst.
@@ -574,39 +552,40 @@ Proof.
     }
     { ss. subst. eexists _, _. splits; eauto. }
     inv STEP_TGT; ss.
-    + inv STEP; ss; try inv STATE.
-      * exploit MemInv.promise; try apply MEMORY; try apply MEM; eauto.
+    + inv STEP; inv STEP0; try inv STATE; ss.
+      * (* promise *)
+        exploit MemInv.promise; try apply MEMORY; eauto.
         { apply WF_SRC. }
         { apply WF_TGT. }
-        i. des. apply MemInv.sem_bot_inv in INV2. subst.
+        s. i. des. apply MemInv.sem_bot_inv in INV2. subst.
         exploit Memory.promise_future; try apply PROMISE_SRC; eauto.
-        { inv WF_SRC. auto. }
+        { apply WF_SRC. }
+        { apply WF_SRC. }
         i. des.
-        eexists _, _, _, _. splits; eauto.
-        { instantiate (1 := Thread.mk _ _ _ _).
-          econs 1. econs 1; s; eauto.
+        eexists _, _, _, _, _, _. splits; eauto.
+        { econs 1. econs 1. econs; s; eauto.
           eapply Commit.future_wf; try apply WF_TGT; eauto.
           etransitivity; eauto. apply Memory.splits_future. inv MEMORY. eauto.
         }
-        { apply rclo5_step. apply ctx_dowhile; auto.
+        { apply rclo7_step. apply ctx_dowhile; auto.
           - apply MemInv.sem_bot.
-          - eapply _sim_stmts_mon; try apply rclo5_incl; eauto.
+          - eapply _sim_stmts_mon; try apply rclo7_incl; eauto.
             eapply _sim_stmts_mon; try apply LE; eauto.
         }
-      * eexists _, _, _, _. splits; eauto.
-        { econs 1. econs 6; eauto. econs.
+      * eexists _, _, _, _, _, _. splits; eauto.
+        { econs 1. econs 2. econs; eauto. s. econs; eauto.
           eapply Commit.future_wf; try apply WF_TGT; eauto.
           apply Memory.splits_future. inv MEMORY. eauto.
         }
-        { apply rclo5_step. eapply ctx_seq.
-          { apply rclo5_incl. apply LE. eauto. }
-          ii. apply rclo5_step. eapply ctx_ite; eauto.
-          - ii. apply rclo5_step. eapply ctx_dowhile; eauto.
-            eapply _sim_stmts_mon; try apply rclo5_incl; eauto.
+        { apply rclo7_step. eapply ctx_seq.
+          { apply rclo7_incl. apply LE. eauto. }
+          ii. apply rclo7_step. eapply ctx_ite; eauto.
+          - ii. apply rclo7_step. eapply ctx_dowhile; eauto.
+            eapply _sim_stmts_mon; try apply rclo7_incl; eauto.
             eapply _sim_stmts_mon; try apply LE; eauto.
-          - ii. apply rclo5_base; auto.
+          - ii. apply rclo7_base; auto.
         }
-    + inv STATE.
+    + inv STEP. inv STATE.
 Qed.
 
 Definition sim_stmts := @_sim_stmts (@sim_thread lang lang).
@@ -627,7 +606,7 @@ Qed.
 Lemma sim_stmts_nil sim_regs:
   sim_stmts sim_regs [] [] sim_regs.
 Proof.
-  ii. pupto5_init. pupto5 ctx_weak_respectful.
+  ii. pupto7_init. pupto7 ctx_weak_respectful.
 Qed.
 
 Lemma sim_stmts_instr
@@ -635,7 +614,7 @@ Lemma sim_stmts_instr
       (REGS: RegSet.disjoint regs (Instr.regs_of instr)):
   sim_stmts (RegFile.eq_except regs) [Stmt.instr instr] [Stmt.instr instr] (RegFile.eq_except regs).
 Proof.
-  ii. pupto5_init. pupto5 ctx_weak_respectful.
+  ii. pupto7_init. pupto7 ctx_weak_respectful.
 Qed.
 
 Lemma sim_stmts_seq
@@ -646,10 +625,10 @@ Lemma sim_stmts_seq
       (SIM2: sim_stmts sim_regs1 stmts2_src stmts2_tgt sim_regs2):
   sim_stmts sim_regs0 (stmts1_src ++ stmts2_src) (stmts1_tgt ++ stmts2_tgt) sim_regs2.
 Proof.
-  ii. pupto5_init. pupto5 ctx_weak_respectful.
+  ii. pupto7_init. pupto7 ctx_weak_respectful.
   econs 4.
-  - pupto5_final. apply SIM1; auto.
-  - ii. pupto5_final. apply SIM2; auto.
+  - pupto7_final. apply SIM1; auto.
+  - ii. pupto7_final. apply SIM2; auto.
 Qed.
 
 Lemma sim_stmts_ite
@@ -661,10 +640,10 @@ Lemma sim_stmts_ite
       (SIM2: sim_stmts sim_regs0 stmts2_src stmts2_tgt sim_regs1):
   sim_stmts sim_regs0 [Stmt.ite cond_src stmts1_src stmts2_src] [Stmt.ite cond_tgt stmts1_tgt stmts2_tgt] sim_regs1.
 Proof.
-  ii. pupto5_init. pupto5 ctx_weak_respectful.
+  ii. pupto7_init. pupto7 ctx_weak_respectful.
   econs 5; eauto.
-  - ii. pupto5_final. apply SIM1; auto.
-  - ii. pupto5_final. apply SIM2; auto.
+  - ii. pupto7_final. apply SIM1; auto.
+  - ii. pupto7_final. apply SIM2; auto.
 Qed.
 
 Lemma sim_stmts_dowhile
@@ -675,6 +654,6 @@ Lemma sim_stmts_dowhile
       (SIM: sim_stmts sim_regs stmts_src stmts_tgt sim_regs):
   sim_stmts sim_regs [Stmt.dowhile stmts_src cond_src] [Stmt.dowhile stmts_tgt cond_tgt] sim_regs.
 Proof.
-  ii. pupto5_init. pupto5 ctx_weak_respectful.
-  econs 6; eauto. ii. pupto5_final. apply SIM; auto.
+  ii. pupto7_init. pupto7 ctx_weak_respectful.
+  econs 6; eauto. ii. pupto7_final. apply SIM; auto.
 Qed.
