src/lib/respectful7.v
@@ -1,0 +1,230 @@
+Require Import paco7.
+Require Import sflib.
+
+Set Implicit Arguments.
+
+Section Respectful7.
+  Variable T0: Type.
+  Variable T1: forall (x0: @T0), Type.
+  Variable T2: forall (x0: @T0) (x1: @T1 x0), Type.
+  Variable T3: forall (x0: @T0) (x1: @T1 x0) (x2: @T2 x0 x1), Type.
+  Variable T4: forall (x0: @T0) (x1: @T1 x0) (x2: @T2 x0 x1) (x3: @T3 x0 x1 x2), Type.
+  Variable T5: forall (x0: @T0) (x1: @T1 x0) (x2: @T2 x0 x1) (x3: @T3 x0 x1 x2) (x4: @T4 x0 x1 x2 x3), Type.
+  Variable T6: forall (x0: @T0) (x1: @T1 x0) (x2: @T2 x0 x1) (x3: @T3 x0 x1 x2) (x4: @T4 x0 x1 x2 x3) (x5: @T5 x0 x1 x2 x3 x4), Type.
+  Definition rel := rel7 T0 T1 T2 T3 T4 T5 T6.
+
+  Variable gf: rel -> rel.
+  Hypothesis gf_mon: monotone7 gf.
+
+  Inductive sound7 (clo: rel -> rel): Prop :=
+  | sound7_intro
+      (MON: monotone7 clo)
+      (SOUND:
+         forall r (PFIX: r <7= gf (clo r)),
+           r <7= paco7 gf bot7)
+  .
+  Hint Constructors sound7.
+
+  Structure respectful7 (clo: rel -> rel) : Prop :=
+  | respectful7_intro
+      (MON: monotone7 clo)
+      (RESPECTFUL:
+         forall l r (LE: l <7= r) (GF: l <7= gf r),
+           clo l <7= gf (clo r)).
+  Hint Constructors respectful7.
+
+  Inductive grespectful7 (r: rel) e1 e2 e3 e4 e5 e6 e7: Prop :=
+  | grespectful7_intro
+      clo
+      (RES: respectful7 clo)
+      (CLO: clo r e1 e2 e3 e4 e5 e6 e7)
+  .
+  Hint Constructors grespectful7.
+
+  Lemma gfclo7_mon: forall clo, sound7 clo -> monotone7 (gf <*> clo).
+  Proof. intros; destruct H; eauto using gf_mon. Qed.
+  Hint Resolve gfclo7_mon : paco.
+
+  Lemma sound7_is_gf: forall clo (UPTO: sound7 clo),
+      paco7 (gf <*> clo) bot7 <7= paco7 gf bot7.
+  Proof.
+    i. punfold PR. edestruct UPTO.
+    eapply (SOUND (paco7 (gf <*> clo) bot7)); eauto.
+    i. punfold PR0.
+    eapply (gfclo7_mon UPTO); eauto.
+    intros. destruct PR1; eauto. done.
+  Qed.
+
+  Lemma respectful7_is_sound7: respectful7 <1= sound7.
+  Proof.
+    intro clo.
+    set (rclo := fix rclo clo n (r: rel) :=
+           match n with
+           | 0 => r
+           | S n' => rclo clo n' r \7/ clo (rclo clo n' r)
+           end).
+    i. destruct PR. econs; eauto.
+    i. set (rr e1 e2 e3 e4 e5 e6 e7 := exists n, rclo clo n r e1 e2 e3 e4 e5 e6 e7).
+    assert (rr x0 x1 x2 x3 x4 x5 x6) by (exists 0; eauto); clear PR.
+    cut (forall n, rclo clo n r <7= gf (rclo clo (S n) r)).
+    { intro X; revert x0 x1 x2 x3 x4 x5 x6 H; pcofix CIH; i.
+      unfold rr in *; des; eauto 10 using gf_mon. }
+    induction n; i; [by s; eauto using gf_mon|].
+    ss; des; [by eauto using gf_mon|].
+    eapply gf_mon; [eapply RESPECTFUL; [|apply IHn|]|]; inst; s; eauto.
+  Qed.
+
+  Lemma respectful7_compose
+        clo1 clo2
+        (RES1: respectful7 clo1)
+        (RES2: respectful7 clo2):
+    respectful7 (clo1 <*> clo2).
+  Proof.
+    i. destruct RES1, RES2.
+    econs.
+    - ii. eapply MON; eauto.
+    - i. eapply RESPECTFUL; [| |apply PR].
+      + i. eapply MON0; eauto.
+      + i. eapply RESPECTFUL0; eauto.
+  Qed.
+
+  Lemma grespectful7_respectful7: respectful7 grespectful7.
+  Proof.
+    econs; ii.
+    - destructs IN RES; exists clo; eauto.
+    - destructs PR RES; eapply gf_mon with (r:=clo r); eauto.
+  Qed.
+
+  Lemma gfgres7_mon: monotone7 (gf <*> grespectful7).
+  Proof.
+    destruct grespectful7_respectful7; eauto using gf_mon.
+  Qed.
+  Hint Resolve gfgres7_mon : paco.
+
+  Lemma grespectful7_greatest: forall clo (RES: respectful7 clo), clo <8= grespectful7.
+  Proof.
+    eauto.
+  Qed.
+
+  Lemma grespectful7_incl: forall r, r <7= grespectful7 r.
+  Proof.
+    i; eexists (fun x => x); eauto.
+  Qed.
+  Hint Resolve grespectful7_incl.
+
+  Lemma grespectful7_compose: forall clo (RES: respectful7 clo) r,
+      clo (grespectful7 r) <7= grespectful7 r.
+  Proof.
+    i; eapply grespectful7_greatest with (clo := clo <*> grespectful7);
+      eauto using respectful7_compose, grespectful7_respectful7.
+  Qed.
+
+  Lemma grespectful7_incl_rev: forall r,
+      grespectful7 (paco7 (gf <*> grespectful7) r) <7= paco7 (gf <*> grespectful7) r.
+  Proof.
+    intro r; pcofix CIH; i; pfold.
+    eapply gf_mon, grespectful7_compose, grespectful7_respectful7.
+    destruct grespectful7_respectful7; eapply RESPECTFUL, PR; i; [by eauto using grespectful7_incl|].
+    punfold PR0.
+      by eapply gfgres7_mon; eauto; i; destruct PR1; eauto.
+  Qed.
+
+  Inductive rclo7 clo (r: rel): rel :=
+  | rclo7_incl
+      e1 e2 e3 e4 e5 e6 e7
+      (R: r e1 e2 e3 e4 e5 e6 e7):
+      @rclo7 clo r e1 e2 e3 e4 e5 e6 e7
+  | rclo7_step'
+      r' e1 e2 e3 e4 e5 e6 e7
+      (R': r' <7= rclo7 clo r)
+      (CLOR':clo r' e1 e2 e3 e4 e5 e6 e7):
+      @rclo7 clo r e1 e2 e3 e4 e5 e6 e7
+  .
+
+  Lemma rclo7_mon clo:
+    monotone7 (rclo7 clo).
+  Proof.
+    ii. induction IN.
+    - econs 1. auto.
+    - econs 2; eauto.
+  Qed.
+  Hint Resolve rclo7_mon: paco.
+
+  Lemma rclo7_base
+        clo
+        (MON: monotone7 clo):
+    clo <8= rclo7 clo.
+  Proof.
+    s. i. econs 2; eauto.
+    eapply MON; eauto. i.
+    econs 1. eauto.
+  Qed.
+
+  Lemma rclo7_step
+        (clo: rel -> rel) r:
+    clo (rclo7 clo r) <7= rclo7 clo r.
+  Proof.
+    i. econs 2; eauto.
+  Qed.
+
+  Lemma rclo7_rclo7
+        clo r
+        (MON: monotone7 clo):
+    rclo7 clo (rclo7 clo r) <7= rclo7 clo r.
+  Proof.
+    i. induction PR; eauto.
+    econs 2; eauto.
+  Qed.
+
+  Structure weak_respectful7 (clo: rel -> rel) : Prop :=
+  | weak_respectful7_intro
+      (MON: monotone7 clo)
+      (RESPECTFUL:
+         forall l r (LE: l <7= r) (GF: l <7= gf r),
+           clo l <7= gf (rclo7 clo r)).
+  Hint Constructors weak_respectful7.
+
+  Lemma weak_respectful7_respectful7
+        clo (RES: weak_respectful7 clo):
+    respectful7 (rclo7 clo).
+  Proof.
+    inv RES. econs; eauto with paco. i.
+    induction PR; i.
+    - eapply gf_mon; eauto. i.
+      apply rclo7_incl. auto.
+    - exploit RESPECTFUL; [|apply H|apply CLOR'|].
+      + i. eapply rclo7_mon; eauto.
+      + i. eapply gf_mon; eauto.
+        apply rclo7_rclo7; auto.
+  Qed.
+
+  Lemma upto7_init:
+      paco7 (gf <*> grespectful7) bot7 <7= paco7 gf bot7.
+  Proof.
+    apply sound7_is_gf; eauto.
+    apply respectful7_is_sound7.
+    apply grespectful7_respectful7.
+  Qed.
+
+  Lemma upto7_final:
+    paco7 gf <8= paco7 (gf <*> grespectful7).
+  Proof.
+    pcofix CIH. i. punfold PR. pfold.
+    eapply gf_mon; [|apply grespectful7_incl].
+    eapply gf_mon; eauto. right. des; auto.
+  Qed.
+
+  Lemma upto7_step
+        r clo (RES: weak_respectful7 clo):
+    clo (paco7 (gf <*> grespectful7) r) <7= paco7 (gf <*> grespectful7) r.
+  Proof.
+    i. apply grespectful7_incl_rev.
+    exploit weak_respectful7_respectful7; eauto. i.
+    eapply grespectful7_greatest; eauto.
+    apply rclo7_base; auto. inv RES. auto.
+  Qed.
+End Respectful7.
+
+Ltac pupto7_init := apply upto7_init; eauto with paco.
+Ltac pupto7_final := apply upto7_final; eauto with paco.
+Ltac pupto7 H := eapply upto7_step; [|exact H|]; eauto with paco.
